src/Std/Classes/Ord/New/LinearPreorder.lean
@@ -1,8 +1,16 @@
 module
 
 prelude
+public import Std.Classes.Ord.Basic
 public import Std.Classes.Ord.New.Preorder
 
 public section
 
-class LawfulLinearPreorder (α : Type u) [Comparable α] extends LawfulPreorder α, LawfulComparable α
+class LawfulLinearPreorder (α : Type u) [Comparable α] extends LawfulPreorder α,
+    LawfulOrientedComparable α
+
+instance (α : Type u) [Ord α] [Comparable α] [LawfulOrd α] [LawfulLinearPreorder α] :
+    Std.TransOrd α where
+  isLE_trans := by
+    simp [Comparable.compare_isLE]
+    apply LawfulPreorder.le_trans
