src/Std/Data/DTreeMap/Internal/Ordered.lean
@@ -7,6 +7,7 @@ prelude
 import Std.Classes.Ord.Basic
 import Std.Data.DTreeMap.Internal.Def
 import Std.Data.Internal.Cut
+import Std.Classes.Ord.New.LinearPreorder
 
 /-!
 # `Ordered` predicate
@@ -26,45 +27,47 @@ namespace Std.DTreeMap.Internal.Impl
 open Std.Internal
 
 /-- Implementation detail of the tree map -/
-def Ordered [Ord α] (t : Impl α β) : Prop :=
-  t.toListModel.Pairwise (fun a b => compare a.1 b.1 = .lt)
+def Ordered [LT α] (t : Impl α β) : Prop :=
+  t.toListModel.Pairwise (fun a b => a.1 < b.1)
 
 /-!
 ## Lemmas about the `Ordered` predicate
 -/
 
-theorem Ordered.left [Ord α] {sz k v l r} (h : (.inner sz k v l r : Impl α β).Ordered) :
+theorem Ordered.left [LT α] {sz k v l r} (h : (.inner sz k v l r : Impl α β).Ordered) :
     l.Ordered :=
   h.sublist (by simp)
 
-theorem Ordered.right [Ord α] {sz k v l r} (h : (.inner sz k v l r : Impl α β).Ordered) :
+theorem Ordered.right [LT α] {sz k v l r} (h : (.inner sz k v l r : Impl α β).Ordered) :
     r.Ordered :=
   h.sublist (by simp)
 
-theorem Ordered.compare_left [Ord α] {sz k v l r} (h : (.inner sz k v l r : Impl α β).Ordered)
-    {k'} (hk' : k' ∈ l.toListModel) : compare k'.1 k = .lt :=
+theorem Ordered.gt_left [LT α] {sz k v l r} (h : (.inner sz k v l r : Impl α β).Ordered)
+    {k'} (hk' : k' ∈ l.toListModel) : k'.1 < k :=
   h.rel_of_mem_append hk' List.mem_cons_self
 
-theorem Ordered.compare_left_beq_gt [Ord α] [TransOrd α] {k : α → Ordering} [IsStrictCut compare k]
+theorem Ordered.compare_left_beq_gt [Ord α] [Comparable α] [LawfulOrd α] [LawfulLinearPreorder α]
+    {k : α → Ordering} [IsStrictCut k]
     {sz k' v' l r} (ho : (.inner sz k' v' l r : Impl α β).Ordered) (hcmp : (k k').isGE)
     (p) (hp : p ∈ l.toListModel) : k p.1 == .gt :=
- beq_iff_eq.2 (IsStrictCut.gt_of_isGE_of_gt hcmp (OrientedCmp.gt_of_lt (ho.compare_left hp)))
+  beq_iff_eq.2 (IsStrictCut.gt_of_isGE_of_gt hcmp (ho.gt_left hp))
 
-theorem Ordered.compare_left_not_beq_eq [Ord α] [TransOrd α] {k : α → Ordering}
-    [IsStrictCut compare k] {sz k' v' l r}
+theorem Ordered.compare_left_not_beq_eq [Ord α] [Comparable α] [LawfulOrd α] [LawfulLinearPreorder α]
+    {k : α → Ordering}
+    [IsStrictCut k] {sz k' v' l r}
     (ho : (.inner sz k' v' l r : Impl α β).Ordered) (hcmp : (k k').isGE)
     (p) (hp : p ∈ l.toListModel) : ¬(k p.1 == .eq) := by
   suffices k p.fst = .gt by simp [this]
-  exact IsStrictCut.gt_of_isGE_of_gt hcmp (OrientedCmp.gt_of_lt (ho.compare_left hp))
+  exact IsStrictCut.gt_of_isGE_of_gt hcmp (ho.gt_left hp)
 
-theorem Ordered.compare_right [Ord α] {sz k v l r}
+theorem Ordered.lt_right [LT α] {sz k v l r}
     (h : (.inner sz k v l r : Impl α β).Ordered) {k'} (hk' : k' ∈ r.toListModel) :
-    compare k k'.1 = .lt := by
+    k < k'.1 := by
   exact List.rel_of_pairwise_cons (h.sublist (List.sublist_append_right _ _)) hk'
 
-theorem Ordered.compare_right_not_beq_gt [Ord α] [TransOrd α] {k : α → Ordering}
-    [IsStrictCut compare k] {sz k' v' l r}
+theorem Ordered.compare_right_not_beq_gt [Ord α] [Comparable α] [LawfulOrd α] [LawfulComparable α]
+    {k : α → Ordering} [IsStrictCut k] {sz k' v' l r}
     (ho : (.inner sz k' v' l r : Impl α β).Ordered) (hcmp : (k k').isLE)
     (p) (hp : p ∈ r.toListModel) : ¬(k p.1 == .gt) := by
   suffices k p.fst = .lt by simp [this]
-  exact IsStrictCut.lt_of_isLE_of_lt hcmp (ho.compare_right hp)
+  exact IsStrictCut.lt_of_isLE_of_lt hcmp (ho.lt_right hp)
