src/Std/Classes/Ord/New/LinearOrder.lean
@@ -7,3 +7,21 @@ public import Std.Classes.Ord.New.PartialOrder
 public section
 
 class LawfulLinearOrder (α : Type u) [Comparable α] extends LawfulLinearPreorder α, LawfulPartialOrder α
+
+instance (α : Type u) [Ord α] [Comparable α] [LawfulOrd α] [LawfulLinearOrder α] :
+    Std.LawfulEqOrd α where
+  eq_of_compare h := by
+    apply LawfulPartialOrder.toAntisymm.antisymm
+    · simp [← Comparable.compare_isLE, h]
+    · rw [Std.OrientedOrd.eq_swap, Ordering.swap_eq_eq] at h
+      simp [← Comparable.compare_isLE, h]
+
+instance (α : Type u) [Comparable α] [LawfulLinearPreorder α] [Std.Antisymm (α := α) (· ≤ ·)] :
+    LawfulLinearOrder α where
+
+instance (α : Type u) [Ord α] [Comparable α] [LawfulOrd α] [LawfulLinearPreorder α]
+    [Std.LawfulEqOrd α] : Std.Antisymm (α := α) (· ≤ ·) where
+  antisymm a b := by
+    cases h : compare a b
+    all_goals simp [← Comparable.compare_isLE, ← Std.LawfulEqOrd.compare_eq_iff_eq (α := α),
+      Std.OrientedOrd.eq_swap (a := b), h]
