src/Std/Classes/Ord/New/PartialOrder.lean
@@ -5,5 +5,5 @@ public import Std.Classes.Ord.New.LinearPreorder
 
 public section
 
-class LawfulPartialOrder (α : Type u) [PartiallyComparable α] extends LawfulPreorder α where
-  le_antisymm : ∀ a b : α, a ≤ b → b ≤ a → a = b
+class LawfulPartialOrder (α : Type u) [PartiallyComparable α] extends LawfulPreorder α,
+    Std.Antisymm (α := α) (· ≤ ·) where
