src/Std/Classes/Ord/New/Preorder.lean
@@ -5,6 +5,16 @@ public import Std.Classes.Ord.New.Comparable
 
 public section
 
-class LawfulPreorder (α : Type u) [PartiallyComparable α] where
+class LawfulPreorder (α : Type u) [PartiallyComparable α] extends LawfulPartiallyComparable α where
   le_trans : ∀ a b c : α, a ≤ b → b ≤ c → a ≤ c
   le_refl : ∀ a : α, a ≤ a
+
+instance (α : Type u) [PartiallyComparable α] [LawfulPreorder α] :
+    Trans (α := α) (· < ·) (· < ·) (· < ·) where
+  trans {a b c} hab hbc := by
+    rw [LawfulPartiallyComparable.lt_iff_le_not_ge] at *
+    constructor
+    · exact LawfulPreorder.le_trans _ _ _ hab.1 hbc.1
+    · intro h
+      have : c ≤ b := LawfulPreorder.le_trans _ _ _ h hab.1
+      exact hbc.2 this
